Upd

temp/Spec.Claim.Capabilities.fst
@@ -8,25 +8,85 @@ open Spec.Claim.Keys
 type key = bytes
 
 assume val sharedSecret : k1: key -> k2: key -> Tot key
+
+
+assume val h1: 'a -> bytes
+assume val h2: 'a -> bytes
 assume val h3: 'a -> bytes
 assume val h4: 'a -> bytes
 
-assume val enc : key: key -> plain : bytes -> Tot bytes
+type kv (a: eqtype) (b:eqtype) = 
+  |MkKV : key: a -> value : b -> kv a b      
+
+assume val vrf: bytes -> (tuple2 (bytes) (bytes))
+assume val enc : key: bytes -> plain: bytes -> Tot(bytes)
+assume val dec: key: bytes -> ciphered: bytes -> Tot bytes
+assume val lemmaEncDec : key: bytes -> plain: bytes -> Lemma (ensures( plain =  (let cipherText = enc key plain in 
+                                                                        dec key cipherText )))
+assume val getTime: unit -> time
 
 
+
+
+val claimEncoding : 
+  privateKeyVRF: bytes -> 
+  nonce: nat -> 
+  claim_label: string -> 
+  claim_body : string -> Tot (tuple2 (bytes) (kv bytes bytes)) 
+
+let claimEncoding privateKeyVRF nonce claim = 
+  let claim_label = getClaimLabel claim in 
+  let claim_body = getClaimBosy claim in 
+  let ncl = concat nonce claim_label in 
+  let k, proof = vrf ncl in 
+  let l = h1 k in 
+  let ke = h2 k in 
+  let c = enc ke (concat proof claim_body) in 
+  (k, MkKV l c)
 
 val encodeCapability : privateKeyDH : key -> 
-		publicKeyReader: key -> 
-		nonce: bytes -> 
-		claimLabel: string -> 
-		k: bytes 0 -> Tot(tuple2 (la: bytes) (pa : bytes))
+        publicKeyReaderDH: key -> 
+        nonce: bytes -> 
+        claimLabel: string -> 
+        k: bytes -> Tot(tuple2 (la: bytes) (pa : bytes))
 
-let encodeCapability privateKeyDH publicKeyReader nonce claimLabel k = 
-	let s = sharedSecret privateKeyDH publicKeyReader in 
-	let claimLabel = toBytes claimLabel in 
-	let la1 = concat nonce s in 
-	let body = concat la1 claimLabel in 
-	let la = h3 body in 
-	let key = h4 body in 
-	let pa = enc key k in 
-	(la, pa)
+let encodeCapability privateKeyOwnerDH publicKeyReaderDH nonce claimLabel k = 
+    let s = sharedSecret privateKeyOwnerDH publicKeyReaderDH in 
+    let claimLabel = toBytes claimLabel in 
+    let la1 = concat nonce s in 
+    let body = concat la1 claimLabel in 
+    let la = h3 body in 
+    let key = h4 body in 
+    let pa = enc key k in 
+(la, pa)
+
+
+val computeCapabilityLookupKey : privateKeyOwnerDH: key -> 
+            publicKeyReaderDH: key -> 
+            nonce: bytes -> 
+            claimLabel : string -> 
+            Tot (lookUpKey : bytes)
+
+let computeCapabilityLookupKey privateKeyOwnerDH publicKeyReaderDH nonce claimLabel = 
+    let s = sharedSecret privateKeyOwnerDH publicKeyReaderDH in 
+    let claimLabel = toBytes claimLabel in 
+    let la1 = concat nonce s in 
+    let body = concat la1 claimLabel in 
+    let la = h3 body in la
+
+val decodeCapability: privateKeyReaderDH: key -> 
+        ownerPublicKeyDH: key -> 
+        nonce : bytes -> 
+        claimLabel : string ->
+        capabilityCiphered: bytes -> 
+        Tot (tuple2 (k: bytes) (l: bytes))
+        
+let decodeCapability privateKeyReaderDH ownerPublicKeyDH nonce claimLabel capabilityCiphered = 
+    let s = sharedSecret privateKeyReaderDH ownerPublicKeyDH in 
+    let claimLabel = toBytes claimLabel in
+    let la1 =  concat nonce s in 
+    let body = concat la1 claimLabel in 
+    let key = h4 body in 
+    let k = dec key capabilityCiphered in 
+    let l = h1 k in 
+    (k, l)
